{
 "cells": [
  {
   "cell_type": "markdown",
   "id": "fdb772ac",
   "metadata": {},
   "source": [
    "## Exercise 5: Function Notation"
   ]
  },
  {
   "cell_type": "markdown",
   "id": "7e564979",
   "metadata": {},
   "source": [
    "> 1. Find and simplify $f(x + 1)$ if $f(x) = 4x − 5$.\n",
    "\n",
    "\\begin{gather*}\n",
    "    f(x) = 4x − 5 \\\\ \\\\\n",
    "    f(x + 1) = 4(x + 1) - 5 \\\\\n",
    "    f(x + 1) = 4x + 4 - 5 \\\\\n",
    "    \\boxed{f(x + 1) = 4x - 1}\n",
    "\\end{gather*}"
   ]
  },
  {
   "cell_type": "markdown",
   "id": "cd89dc94",
   "metadata": {},
   "source": [
    "> 2. What went wrong in this set of steps?\n",
    "\n",
    "\\begin{gather*}\n",
    "    \\text{Evaluate } f(x) = x^2 \\text{ at } x = -2 \\\\ \\\\\n",
    "    f(-2) = -2^2 + 1 \\\\\n",
    "    f(-2) = -4 + 1 \\\\\n",
    "    f(-2) = -3 \\\\\n",
    "\\end{gather*}\n",
    "\n",
    "In the first step, the $-2$ in $-2^2$ should be enclosed and written like this: $(-2)^2$ and the answer should be $4$ instead of $-4$."
   ]
  },
  {
   "cell_type": "markdown",
   "id": "ab007ff9",
   "metadata": {},
   "source": [
    "> 3. Find and simplify $h(s^2)$ if $h(s) = −s^2 + 3s − 1$.\n",
    "\n",
    "\\begin{gather*}\n",
    "    h(s) = −s^2 + 3s − 1 \\\\ \\\\\n",
    "    h(s^2) = -(s^2)^2 + 3(s^2) - 1 \\\\\n",
    "    \\boxed{h(s^2) = -s^4 + 3s^2 - 1}\n",
    "\\end{gather*}"
   ]
  },
  {
   "cell_type": "markdown",
   "id": "530779e8",
   "metadata": {},
   "source": [
    "> 4. If $g(x) = x3 − x + 1$, what do we need to plug into the function in order\n",
    "to get the following expression?\n",
    "\n",
    "\\begin{gather*}\n",
    "    g(??) = (2x + 1)^3 - (2x + 1) + 1 \\\\\n",
    "\\end{gather*}\n",
    "\n",
    "The value we need to plug is $2x + 1$.\n"
   ]
  },
  {
   "cell_type": "markdown",
   "id": "24b3ccc4",
   "metadata": {},
   "source": [
    "> 5. Find the value of the expression if $f(x) = x^2 + x − 1$.\n",
    "\n",
    "\\begin{gather*}\n",
    "    \\frac{f(x + h) - f(x)}{h} \\\\ \\\\\n",
    "\n",
    "    f(x + h) = (x + h)^2 + (x + h) - 1 \\\\\n",
    "    f(x + h) = x^2 + 2hx + h^2 + x + h - 1 \\\\ \\\\\n",
    "\n",
    "    \\frac{x^2 + 2hx + h^2 + x + h - 1 - (x^2 + x - 1)}{h} \\\\\n",
    "    \\frac{x^2 + 2hx + h^2 + x + h - 1 - x^2 - x + 1}{h} \\\\\n",
    "    \\frac{2hx + h^2 + h}{h} \\\\\n",
    "    \\boxed{2x + h + 1}\n",
    "\\end{gather*}\n"
   ]
  },
  {
   "cell_type": "markdown",
   "id": "eb9219a3",
   "metadata": {},
   "source": [
    "> 6. What went wrong in this set of steps?\n",
    "\n",
    "\\begin{gather*}\n",
    "    \\text{Find } f(1) \\text{ if } f(x) = x^3 + 3x^2 - 5x + 2. \\\\ \\\\\n",
    "    f(1) = 1^3 + 3(1)^2 - 5(1) + 2 \\\\\n",
    "    f(1) = 1 + 9 - 5 + 2 \\\\\n",
    "    f(1) = 7\n",
    "\\end{gather*}\n",
    "\n",
    "In the second step, $3(1)^2$ should result in $3$ instead of $9$"
   ]
  }
 ],
 "metadata": {
  "language_info": {
   "name": "python"
  }
 },
 "nbformat": 4,
 "nbformat_minor": 5
}
