{
 "cells": [
  {
   "cell_type": "markdown",
   "id": "f6a5c2e6",
   "metadata": {},
   "source": [
    "## Exercise 5: Systems with Non-Linear Equations"
   ]
  },
  {
   "cell_type": "markdown",
   "id": "1792f880",
   "metadata": {},
   "source": [
    "> 1. Solve the system of equations.\n",
    "\n",
    "\\begin{gather*}\n",
    "    y = x - 1 \\\\\n",
    "    x^2 + y^2 = 1 \\\\ \\\\\n",
    "\n",
    "    x^2 + (x - 1)^2 = 1 \\\\\n",
    "    x^2 + (x - 1)(x - 1) = 1 \\\\\n",
    "    x^2 + x^2 - 2x + 1 = 1 \\\\\n",
    "    2x^2 - 2x = 1 - 1 \\\\\n",
    "    2x^2 - 2x = 0 \\\\\n",
    "    x^2 - x = 0 \\\\\n",
    "    x(x - 1) = 0 \\\\\n",
    "    x = 0, 1 \\\\ \\\\\n",
    "\n",
    "    y = 0 - 1 \\\\\n",
    "    y = -1 \\\\ \\\\\n",
    "\n",
    "    \\boxed{(0, -1)} \\\\ \\\\\n",
    "\n",
    "    y = 1 - 1 \\\\\n",
    "    y = 0 \\\\ \\\\\n",
    "\n",
    "    \\boxed{(1, 0)}\n",
    "\\end{gather*}"
   ]
  },
  {
   "cell_type": "markdown",
   "id": "4591f17c",
   "metadata": {},
   "source": [
    "> 2. Solve the system of equations.\n",
    "\n",
    "\\begin{gather*}\n",
    "    y - 2x = 0 \\\\\n",
    "    (x - 2)^2 + (y - 1)^2 = 9 \\\\ \\\\\n",
    "\n",
    "    y = 2x \\\\ \\\\\n",
    "\n",
    "    (x - 2)^2 + (2x - 1)^2 = 9 \\\\\n",
    "    x^2 - 4x + 4 + 4x^2 - 4x + 1 = 9 \\\\\n",
    "    5x^2 - 8x + 5 = 9 \\\\\n",
    "    5x^2 - 8x - 4 = 0 \\\\ \\\\\n",
    "\n",
    "    5 \\cdot -4 = -20 \\\\\n",
    "    a + b = -8 \\\\\n",
    "    a \\cdot b = -20 \\\\\n",
    "    -10 + 2 = -8 \\\\\n",
    "    -10 \\cdot 2 = -20 \\\\ \\\\\n",
    "\n",
    "    5x^2 - 10x + 2x - 4 \\\\\n",
    "    (5x^2 - 10x) + (2x - 4) \\\\\n",
    "    5x(x - 2) + 2(x - 2) \\\\\n",
    "    (5x + 2)(x - 2) = 0 \\\\\n",
    "    x = -\\frac{2}{5}, 2 \\\\ \\\\\n",
    "\n",
    "    y = 2(-\\frac{2}{5}) \\\\\n",
    "    y = -\\frac{4}{5} \\\\ \\\\\n",
    "\n",
    "    \\boxed{\\left(-\\frac{2}{5}, -\\frac{4}{5}\\right)} \\\\ \\\\\n",
    "\n",
    "    y = 2(2) \\\\\n",
    "    y = 4 \\\\ \\\\\n",
    "\n",
    "    \\boxed{(2, 4)}\n",
    "\\end{gather*}"
   ]
  },
  {
   "cell_type": "markdown",
   "id": "44ee05d6",
   "metadata": {},
   "source": [
    "> 3. Solve the system of equations.\n",
    "\n",
    "\\begin{gather*}\n",
    "    2y − x = − 2 \\\\\n",
    "    (x − 6)^2 + 4(y − 4)^2 = 16 \\\\ \\\\\n",
    "\n",
    "    x = 2y + 2 \\\\ \\\\\n",
    "\n",
    "    (2y + 2 - 6)^2 + 4(y - 4)^2 = 16 \\\\\n",
    "    (2y - 4)^2 + 4(y^2 - 8x + 16) = 16 \\\\\n",
    "    4y^2 - 16y + 16 + 4(y^2 - 8x + 16) = 16 \\\\\n",
    "    \\frac{4y^2 - 16y + 16 + 4(y^2 - 8x + 16) = 16}{4} \\\\\n",
    "    y^2 - 4y + 4 + y^2 - 8x + 16 = 4 \\\\\n",
    "    2y^2 - 12y + 16 = 0 \\\\\n",
    "    y^2 - 6y + 8 = 0 \\\\\n",
    "    (y - 4)(y - 2) = 0 \\\\\n",
    "    y = 4, 2 \\\\ \\\\\n",
    "\n",
    "    x = 2(4) + 2 \\\\\n",
    "    x = 8 + 2 \\\\\n",
    "    x = 10 \\\\ \\\\\n",
    "\n",
    "    \\boxed{(10, 4)} \\\\ \\\\\n",
    "\n",
    "    x = 2(2) + 2 \\\\\n",
    "    x = 4 + 2 \\\\\n",
    "    x = 6 \\\\ \\\\\n",
    "\n",
    "    \\boxed{(6, 2)}\n",
    "\\end{gather*}"
   ]
  },
  {
   "cell_type": "markdown",
   "id": "e0cd5eb5",
   "metadata": {},
   "source": [
    "> 4. Solve the system of equations.\n",
    "\n",
    "\\begin{gather*}\n",
    "    y = \\frac{1}{2}x + 1 \\\\\n",
    "    x^2 − y^2 = 4 \\\\ \\\\\n",
    "\n",
    "    x^2 - (\\frac{1}{2}x + 1)^2 = 4 \\\\\n",
    "    x^2 - (\\frac{1}{2}x + 1)(\\frac{1}{2}x + 1) = 4 \\\\\n",
    "    x^2 - (\\frac{1}{4}x^2 + x + 1) = 4 \\\\\n",
    "    x^2 - \\frac{1}{4}x^2 - x - 1 = 4 \\\\\n",
    "    \\frac{3}{4}x^2 - x - 1 = 4 \\\\\n",
    "    4\\left(\\frac{3}{4}x^2 - x - 1 = 4\\right) \\\\\n",
    "    3x^2 - 4x - 4 = 16 \\\\\n",
    "    3x^2 - 4x - 4 - 16 = 0 \\\\\n",
    "    3x^2 - 4x - 20 = 0 \\\\ \\\\\n",
    "\n",
    "    3 \\cdot -20 = -60 \\\\\n",
    "    a + b = -4 \\\\\n",
    "    a \\cdot b = -60 \\\\\n",
    "    -10 + 6 = -4 \\\\\n",
    "    -10 \\cdot 6 = -60 \\\\ \\\\\n",
    "\n",
    "    3x^2 + 6x - 10x - 20 \\\\\n",
    "    (3x^2 + 6x) - (10x - 20) \\\\\n",
    "    3x(x + 2) - 10(x + 2) \\\\\n",
    "    (3x - 10)(x + 2) \\\\ \n",
    "    x = \\frac{10}{3}, -2 \\\\ \\\\\n",
    "\n",
    "    y = \\frac{1}{2}(\\frac{10}{3}) + 1 \\\\\n",
    "    y = \\frac{10}{6} + 1 \\\\\n",
    "    y = \\frac{5}{3} + \\frac{3}{3} \\\\\n",
    "    y = \\frac{8}{3} \\\\ \\\\\n",
    "\n",
    "    \\boxed{(x, y) = (\\frac{10}{3}, \\frac{8}{3})} \\\\ \\\\\n",
    "\n",
    "    y = \\frac{1}{2}(-2) + 1 \\\\\n",
    "    y = -1 + 1 \\\\\n",
    "    y = 0 \\\\ \\\\\n",
    "\n",
    "    \\boxed{(x, y) = (-2, 0)}\n",
    "\\end{gather*}"
   ]
  },
  {
   "cell_type": "markdown",
   "id": "0cc45365",
   "metadata": {},
   "source": [
    "> 5. Solve the system of equations.\n",
    "\n",
    "\\begin{gather*}\n",
    "    y = -\\frac{1}{2}x - 3 \\\\ \n",
    "    \\frac{(x - 3)^2}{9} - \\frac{(y + 3)^2}{9} = 1 \\\\ \\\\\n",
    "\n",
    "    \\frac{(x - 3)^2}{9} - \\frac{(-\\frac{1}{2}x - 3 + 3)^2}{9} = 1 \\\\\n",
    "    9\\left(\\frac{(x - 3)^2}{9} - \\frac{(-\\frac{1}{2}x - 3 + 3)^2}{9} = 1\\right) \\\\\n",
    "    (x - 3)^2 - (-\\frac{1}{2}x)^2 = 9 \\\\\n",
    "    (x - 3)(x - 3) - (-\\frac{1}{2}x)(-\\frac{1}{2}x) = 9 \\\\\n",
    "    x^2 - 6x + 9 - (\\frac{1}{4}x^2) = 9 \\\\\n",
    "    x^2 - 6x + 9 - \\frac{1}{4}x^2 = 9 \\\\\n",
    "    \\frac{3}{4}x^2 - 6x + 9 = 9 \\\\\n",
    "    4\\left(\\frac{3}{4}x^2 - 6x + 9 = 9\\right) \\\\\n",
    "    3x^2 - 24x + 36 = 36 \\\\\n",
    "    3x^2 - 24x + 36 - 36 = 0 \\\\\n",
    "    3x^2 - 24x = 0 \\\\\n",
    "    3x(x - 8) = 0 \\\\\n",
    "    x = 0, 8 \\\\ \\\\\n",
    "\n",
    "    y = -\\frac{1}{2}(0) - 3 \\\\\n",
    "    y = -3 \\\\ \\\\\n",
    "\n",
    "    \\boxed{(x, y) = (0, -3)} \\\\ \\\\\n",
    "\n",
    "    y = -\\frac{1}{2}(8) - 3 \\\\\n",
    "    y = -4 - 3 \\\\\n",
    "    y = -7 \\\\ \\\\\n",
    "\n",
    "    \\boxed{(x, y) = (8, -7)}\n",
    "\\end{gather*}"
   ]
  },
  {
   "cell_type": "markdown",
   "id": "95c95494",
   "metadata": {},
   "source": [
    "> 6. Solve the system of equations.\n",
    "\n",
    "\\begin{gather*}\n",
    "    2y - 3x = 14 \\\\\n",
    "    \\frac{(y + 2)^2}{9} + \\frac{(x + 4)^2}{4} = 1 \\\\ \\\\\n",
    "\n",
    "    2y = 3x + 14 \\\\\n",
    "    \\frac{2y = 3x + 14}{2} \\\\\n",
    "    y = \\frac{3}{2}x + 7 \\\\ \\\\\n",
    "\n",
    "    \\frac{(\\frac{3}{2}x + 7 + 2)^2}{9} + \\frac{(x + 4)^2}{4} = 1 \\\\\n",
    "    36\\left(\\frac{(\\frac{3}{2}x + 7 + 2)^2}{9} + \\frac{(x + 4)^2}{4} = 1\\right) \\\\\n",
    "    4(\\frac{3}{2}x + 7 + 2)^2 + 9(x + 4)^2 = 36 \\\\\n",
    "    4(\\frac{3}{2}x + 9)(\\frac{3}{2}x + 9) + 9(x + 4)(x + 4) = 36 \\\\\n",
    "    4(\\frac{9}{4}x^2 + 27x + 81) + 9(x^2 + 8x + 16) = 36 \\\\\n",
    "    9x^2 + 108x + 324 + 9x^2 + 72x + 144 = 36 \\\\\n",
    "    18x^2 + 180x + 468 = 36 \\\\\n",
    "    18x^2 + 180x + 468 - 36 = 0 \\\\\n",
    "    18x^2 + 180x + 432 = 0 \\\\\n",
    "    \\frac{18x^2 + 180x + 432 = 0}{18} \\\\\n",
    "    x^2 + 10x + 24 = 0 \\\\\n",
    "    (x + 6)(x + 4) = 0 \\\\\n",
    "    x = -6, -4 \\\\ \\\\\n",
    "\n",
    "    y = \\frac{3}{2}(-6) + 7 \\\\\n",
    "    y = -\\frac{18}{2} + 7 \\\\\n",
    "    y = -9 + 7 \\\\\n",
    "    y = -2 \\\\ \\\\\n",
    "\n",
    "    \\boxed{(x, y) = (-6, -2)} \\\\ \\\\\n",
    "\n",
    "    y = \\frac{3}{2}(-4) + 7 \\\\\n",
    "    y = -\\frac{12}{2} + 7 \\\\\n",
    "    y = -6 + 7 \\\\\n",
    "    y = 1 \\\\ \\\\\n",
    "\n",
    "    \\boxed{(x, y) = (-4, 1)}\n",
    "\\end{gather*}"
   ]
  }
 ],
 "metadata": {
  "language_info": {
   "name": "python"
  }
 },
 "nbformat": 4,
 "nbformat_minor": 5
}
