{
 "cells": [
  {
   "cell_type": "markdown",
   "id": "df053cef",
   "metadata": {},
   "source": [
    "## Quiz 95: Systems of Three Equations"
   ]
  },
  {
   "cell_type": "markdown",
   "id": "4d5188d5",
   "metadata": {},
   "source": [
    "> 1. Use any method to find the solution to the system of equations. \n",
    "\n",
    "\\begin{gather*}\n",
    "    x + y - z = 4 \\\\\n",
    "    x - y - z = 2 \\\\\n",
    "    x + 2y + z = 1 \\\\ \\\\\n",
    "\n",
    "    x + y - z = 4 \\\\\n",
    "    + (x - y - z = 2) \\\\ \\\\\n",
    "\n",
    "    2x - 2z = 6 \\\\\n",
    "    \\frac{2x - 2z = 6}{2} \\\\\n",
    "    x - z = 3 \\\\ \\\\\n",
    "\n",
    "    2(x - y - z = 2) \\\\\n",
    "    + (x + 2y + z = 1) \\\\ \\\\\n",
    "\n",
    "    2x - 2y - 2z = 4 \\\\\n",
    "    + (x + 2y + z = 1) \\\\\n",
    "    3x - z = 5 \\\\ \\\\\n",
    "\n",
    "    -3(x - z = 3) \\\\\n",
    "    + (3x - z = 5) \\\\ \\\\\n",
    "\n",
    "    -3x + 3z = -9 \\\\\n",
    "    + (3x - z = 5) \\\\\n",
    "    2z = -4 \\\\\n",
    "    \\frac{2z = -4}{2} \\\\\n",
    "    \\boxed{z = -2} \\\\ \\\\\n",
    "\n",
    "    x - z = 3 \\\\\n",
    "    x - (-2) = 3 \\\\\n",
    "    x + 2 = 3 \\\\\n",
    "    x = 3 - 2 \\\\\n",
    "    \\boxed{x = 1} \\\\ \\\\\n",
    "\n",
    "    x + y - z = 4 \\\\\n",
    "    (1) + y - (-2) = 4 \\\\\n",
    "    1 + y + 2 = 4 \\\\\n",
    "    y + 3 = 4 \\\\\n",
    "    y = 4 - 3 \\\\\n",
    "    \\boxed{y = 1} \\\\ \\\\\n",
    "\n",
    "    \\textbf{CHECKING} \\\\\n",
    "    x + y - z = 4 \\\\\n",
    "    (1) + (1) - (-2) = 4 \\\\\n",
    "    2 + 2 = 4 \\\\\n",
    "    4 = 4 \\\\ \\\\\n",
    "\n",
    "    x - y - z = 2 \\\\\n",
    "    (1) - (1) - (-2) = 2\\\\\n",
    "    0 + 2 = 2 \\\\\n",
    "    2 + 2 \\\\ \\\\\n",
    "\n",
    "    x + 2y + z = 1 \\\\\n",
    "    (1) + 2(1) + (-2) = 1 \\\\\n",
    "    1 + 2 - 2 = 1 \\\\\n",
    "    1 = 1\n",
    "\\end{gather*}"
   ]
  },
  {
   "cell_type": "markdown",
   "id": "d1519acd",
   "metadata": {},
   "source": [
    "> 2. Use any method to find the solution to the system of equations. \n",
    "\n",
    "\\begin{gather*}\n",
    "    x - y + z = -6 \\\\\n",
    "    3x - 4y - z = -4 \\\\\n",
    "    -2x + 3y + 4z = 14 \\\\ \\\\\n",
    "\n",
    "    x = y - z - 6 \\\\\n",
    "    3(y - z - 6) - 4y - z = -4 \\\\\n",
    "    3y - 3z - 18 - 4y - z = -4 \\\\\n",
    "    -y - 4z - 18 = -4 \\\\\n",
    "    -y - 4z = -4 + 18 \\\\\n",
    "    -y - 4z = 14 \\\\\n",
    "    y = -4z - 14 \\\\ \\\\\n",
    "\n",
    "    x = y - z - 6 \\\\\n",
    "    x = (-4z - 14) - z - 6 \\\\\n",
    "    x = -4z - 14 - z - 6 \\\\\n",
    "    x = -5z - 20 \\\\ \\\\\n",
    "\n",
    "    -2x + 3y + 4z = 14 \\\\\n",
    "    -2(-5z - 20) + 3(-4z - 14) + 4z = 14\n",
    "    10z + 40 - 12z - 42 + 4z = 14 \\\\\n",
    "    10z - 12z + 4z + 40 - 42 = 14 \\\\\n",
    "    2z - 2 = 14 \\\\\n",
    "    2z = 14 + 2 \\\\\n",
    "    2z = 16 \\\\\n",
    "    \\frac{2z = 16}{2} \\\\\n",
    "    \\boxed{z = 8} \\\\ \\\\\n",
    "\n",
    "    x = -5z - 20 \\\\\n",
    "    x = -5(8) - 20 \\\\\n",
    "    x = -40 - 20 \\\\\n",
    "    \\boxed{x = -60} \\\\ \\\\\n",
    "\n",
    "    x - y + z = -6 \\\\\n",
    "    (-60) - y + (8) = -6 \\\\\n",
    "    -52 - y = -6 \\\\\n",
    "    \\boxed{y = -46} \\\\ \\\\\n",
    "\n",
    "    \\textbf{CHECKING} \\\\\n",
    "    x - y + z = -6 \\\\\n",
    "    (-60) - (-46) + 8 = -6 \\\\\n",
    "    -60 + 46 + 8 = -6 \\\\\n",
    "    -14 + 8 = -6 \\\\\n",
    "    -6 = -6 \\\\ \\\\\n",
    "\n",
    "    3x - 4y - z = -4 \\\\\n",
    "    3(-60) - 4(-46) - (8) = -4 \\\\\n",
    "    -180 + 184 - 8 = -4 \\\\\n",
    "    4 - 8 = -4 \\\\\n",
    "    -4 = -4 \\\\ \\\\\n",
    "\n",
    "    -2x + 3y + 4z = 14 \\\\\n",
    "    -2(-60) + 3(-46) + 4(8) = 14 \\\\\n",
    "    120 - 138 + 32 = 14 \\\\\n",
    "    -18 + 32 = 14 \\\\\n",
    "    14 = 14\n",
    "\\end{gather*}"
   ]
  },
  {
   "cell_type": "markdown",
   "id": "efec50d3",
   "metadata": {},
   "source": [
    "> 3. Solve this system of equations for $x$, $y$, and $z$. \n",
    "\n",
    "\\begin{gather*}\n",
    "    x + 2z = 3 \\\\\n",
    "    3x - 2y + z = -11 \\\\\n",
    "    2x + y + 3z = 9 \\\\ \\\\\n",
    "\n",
    "    x = 3 - 2z \\\\ \\\\\n",
    "\n",
    "    3(3 - 2z) - 2y + z = -11 \\\\\n",
    "    9 - 6z - 2y + z = - 11 \\\\\n",
    "    -5z - 2y = -11 - 9 \\\\\n",
    "    -5z - 2y = -20\n",
    "\n",
    "    2x + y + 3z = 9 \\\\\n",
    "    2(3 - 2z) + y + 3z = 9 \\\\\n",
    "    6 - 4z + y + 3z = 9 \\\\\n",
    "    -z + y = 9 - 6 \\\\\n",
    "    -z + y = 3 \\\\\n",
    "\n",
    "    -5z - 2y = -20 \\\\\n",
    "    + (-z + y = 3) \\\\ \\\\\n",
    "\n",
    "    -5z - 2y = -20 \\\\\n",
    "    + 2(-z + y = 3) \\\\ \\\\\n",
    "\n",
    "    -5z - 2y = -20 \\\\\n",
    "    + -2z + 2y = 6 \\\\ \\\\\n",
    "\n",
    "    -7z = -14 \\\\\n",
    "    \\frac{-7z = -14}{-7} \\\\\n",
    "    \\boxed{z = 2} \\\\ \\\\\n",
    "\n",
    "    x = 3 - 2z \\\\\n",
    "    x = 3 - 2(2) \\\\\n",
    "    x = 3 - 4 \\\\\n",
    "    \\boxed{x = -1} \\\\ \\\\\n",
    "\n",
    "    3x - 2y + z = -11 \\\\\n",
    "    3(-1) - 2y + (2) = -11 \\\\\n",
    "    -3 - 2y + 2 = -11 \\\\\n",
    "    -1 - 2y = -11 \\\\\n",
    "    -2y = -11 + 1 \\\\\n",
    "    -2y = -10 \\\\\n",
    "    \\frac{-2y = -10}{-2} \\\\\n",
    "    \\boxed{y = 5} \\\\ \\\\\n",
    "\n",
    "    \\textbf{CHECKING} \\\\\n",
    "    x + 2z = 3 \\\\\n",
    "    (-1) + 2(2) = 3 \\\\\n",
    "    -1 + 4 = 3 \\\\\n",
    "    3 = 3 \\\\ \\\\\n",
    "\n",
    "    3x - 2y + z = -11 \\\\\n",
    "    3(-1) - 2(5) + (2) = -11 \\\\\n",
    "    -3 - 10 + 2 = - 11 \\\\\n",
    "    -13 + 2 = -11 \\\\\n",
    "    -11 = -11 \\\\ \\\\\n",
    "\n",
    "    2x + y + 3z = 9 \\\\\n",
    "    2(-1) + (5) + 3(2) = 9 \\\\\n",
    "    -2 + 5 + 6 = 9 \\\\\n",
    "    3 + 6 = 9 \\\\\n",
    "    9 = 9 \n",
    "\\end{gather*}"
   ]
  }
 ],
 "metadata": {
  "language_info": {
   "name": "python"
  }
 },
 "nbformat": 4,
 "nbformat_minor": 5
}
